Update to nat_indexed based CTL lib

src/AttarchProperties.v
@@ -9,22 +9,19 @@ Open Scope string_scope.
 Open Scope tprop_scope.
 Open Scope env_scope.
 
-Definition useram_key_secure : tprop attarch_state := ⟨λ '(l, _),
+Definition useram_key_secure : tprop attarch_state := <[λ '(l, _),
     forall Γ l' s c,
       l = sel4_run (l', Γ) s ->
       read Γ c "useram_key" good_useram_key -> 
       c = "useram"
-  ⟩.
+  ]>.
 
 Definition diverged : tprop attarch_state :=
-  ⟨λ '(l, _), l = attarch_bot⟩.
+  <[λ '(l, _), l = attarch_bot]>.
 
 Ltac star_notation := 
   repeat change (clos_refl_trans_n1 _ ?R) with (R^*) in *.
 
-(* AG strong induction. Reflect to seq. Hypothesis 
-   is in_seq x -> R @ x ⊨ H
- *)
 
 Theorem useram_key_never_compromised:
   attarch_trans @attarch_init_state ⊨ AG useram_key_secure.
@@ -32,35 +29,73 @@ Proof.
   apply star__AG.
   intros * Hstar.
   induct! Hstar; star_notation.
-  - tentails!. discriminate.
+  - follows tentails!.
   - invc H.
     + tentails!.
-      intros * [=] H'; subst.
-      econtradiction no_lookup_no_read; [|eassumption].
-      now unfold map_access.
+      intros * [=] H'; subst!.
+      follows econtradiction no_lookup_no_read.
     + tentails!.
-      intros * [=] H'; subst.
-      econtradiction no_lookup_no_read; [|eassumption].
-      now unfold map_access.
+      intros * [=] H'; subst!.
+      follows econtradiction no_lookup_no_read.
     + invc H.
       * tentails! in *.
-        intros * [=] H'; subst.
+        intros * [=] H'; subst!.
         eapply IHHstar.
-        reflexivity.
-        eapply write_unchanged_read'; try eassumption.
-        discriminate.
+       -- reflexivity.
+       -- follows eapply write_unchanged_read'.
       * tentails! in *.
-        intros * [=] H'; subst.
-        now eapply IHHstar.
+        intros * [=] H'; subst!.
+        follows eapply IHHstar.
     + invc H.
       invc H0.
       tentails! in *.
-      intros * [=] H'; subst.
-      now eapply IHHstar.
-    + now tentails!.
+      intros * [=] H'; subst!.
+      follows eapply IHHstar.
+    + follows tentails!.
 Qed.
-Print Assumptions useram_key_never_compromised.
+(* Print Assumptions useram_key_never_compromised. *)
 
+
+Theorem useram_key_never_compromised':
+  attarch_trans @attarch_init_state ⊨ A[useram_key_secure W diverged].
+Proof.
+  apply AW_intro; split.
+  - left. follows tentails!.
+  - intros s' seq IH s'' step.
+    invc step.
+    + left.
+      tentails!.
+      intros * [=] H'; subst!.
+      follows econtradiction no_lookup_no_read.
+    + left.
+      tentails!.
+      intros * [=] H'; subst!.
+      follows econtradiction no_lookup_no_read.
+    + left.
+      invc H.
+      * especialize IH; forward IH by apply in_seq_head.
+        destruct IH as [IH _].
+        tentails! in *.
+        intros * [=] H'; subst!.
+        eapply IH; [reflexivity|].
+        follows eapply write_unchanged_read'.
+      * especialize IH; forward IH by apply in_seq_head.
+        destruct IH as [IH _].
+        tentails! in *.
+        intros * [=] H'; subst!.
+        follows eapply IH.
+    + left.
+      invc H.
+      invc H0.
+      especialize IH; forward IH by apply in_seq_head.
+      destruct IH as [IH _].
+      tentails! in *.
+      intros * [=] H'; subst!.
+      follows eapply IH.
+    + right.
+      follows tentails!.
+Qed.
+(* Print Assumptions useram_key_never_compromised'. *)
 
 Close Scope tprop_scope.
 Close Scope string_scope.
